examples: Use defn! notation in most examples

src/Rupicola/Examples/Cells/Swap.v
@@ -5,26 +5,28 @@ Section with_parameters.
   Context {semantics : Semantics.parameters}
           {semantics_ok : Semantics.parameters_ok semantics}.
 
-  Definition swap_gallina_spec (c1 c2: cell) :=
+  Definition swap_gallina (c1 c2: cell) :=
     let/n v1 := get c1 in
     let/n v2 := get c2 in
     let/n c1 := put v2 c1 in
     let/n c2 := put v1 c2 in
     (c1, c2).
 
+  Instance spec_of_swap : spec_of "swap" :=
+    fun functions =>
+      forall c1_ptr c1 c2_ptr c2 tr R mem,
+        sep (TwoCells c1_ptr c2_ptr (c1, c2) []) R mem ->
+        WeakestPrecondition.call
+          functions
+          "swap"
+          tr mem [c1_ptr; c2_ptr]
+          (postcondition_func_norets
+             (TwoCells c1_ptr c2_ptr (swap_gallina c1 c2))
+             R tr).
+
   Derive swap_body SuchThat
-         (let swap := ("swap", (["c1"; "c2"], [], swap_body)) in
-          program_logic_goal_for swap
-          (forall functions,
-           forall c1_ptr c1 c2_ptr c2 tr R mem,
-             sep (TwoCells c1_ptr c2_ptr (c1, c2) []) R mem ->
-             WeakestPrecondition.call
-               (swap :: functions)
-               "swap"
-               tr mem [c1_ptr; c2_ptr]
-               (postcondition_func_norets
-                  (TwoCells c1_ptr c2_ptr (swap_gallina_spec c1 c2))
-                  R tr)))
+         (defn! "swap"("c1", "c2") { swap_body },
+          implements swap_gallina)
     As swap_body_correct.
   Proof.
     compile.
